sfi/refinementSA.v
@@ -16,6 +16,8 @@ Section RefinementSA.
 Set Implicit Arguments.
 
 Import PartMaps.
+Import Abs.Notations.
+Import Abs.Hints.
 Import Sym.EnhancedDo.
 
 (* I want to use S and I as variables. *)
@@ -35,15 +37,18 @@ Notation word    := (word t).
 Notation stag    := (@Sym.stag t).
 Notation sym_sfi := (@Sym.sym_sfi t ops).
 
+Notation satom  := (atom word stag).
+Notation svalue := (@val word stag).
+Notation slabel := (@common.tag word stag).
+
 Notation astate := (@Abs.state t).
 Notation sstate := (@Symbolic.state t sym_sfi).
 
 Notation astep := Abs.step.
 Notation sstep := Sym.step.
 
-Notation satom  := (atom word stag).
-Notation svalue := (@val word stag).
-Notation slabel := (@common.tag word stag).
+Hint Immediate word_map_axioms.
+Hint Immediate reg_map_axioms.
 
 (* We check the compartment stuff later *)
 Definition refine_pc_b (apc : word) (spc : satom) :=
@@ -65,43 +70,46 @@ Definition refine_reg_b (ar : word) (sr : satom) : bool :=
     | _             => false
   end.
 
-Definition refine_memory : Abs.memory t -> Sym.memory t -> Prop :=
+Definition refine_memory : memory t -> Sym.memory t -> Prop :=
   pointwise refine_mem_loc_b.
 
-Definition refine_registers : Abs.registers t -> Sym.registers t -> Prop :=
+Definition refine_registers : registers t -> Sym.registers t -> Prop :=
   pointwise refine_reg_b.
 
-Section With_EqType_refine_compartment_b.
+Section With_EqType_refined_compartment.
 Import Sym.
-Definition refine_compartment_b (c : Abs.compartment t)
-                                (smem : Sym.memory t) : bool :=
-  is_some $
-    let: Abs.Compartment A J S := c in
-    do! sxs <- map_options (get smem) A;
-    do! sc  <- the =<< map_options (stag_compartment ∘ slabel) sxs;
-               (* modulo emptiness *)
-    do! guard? forallb (set_elem sc) <$>
-                 map_options (stag_incoming ∘ slabel <=< get smem) J;
-    do! guard? forallb (set_elem sc) <$>
-                 map_options (stag_writers  ∘ slabel <=< get smem) S;
-    Some tt.
-End With_EqType_refine_compartment_b.
+Definition refined_compartment (c    : Abs.compartment t)
+                               (smem : Sym.memory t) : option word :=
+  let: <<A,J,S>> := c in
+  do! sxs <- map_options (get smem) A;
+  do! sc  <- the =<< map_options (stag_compartment ∘ slabel) sxs;
+             (* modulo emptiness *)
+  do! guard? forallb (set_elem sc) <$>
+               map_options (stag_incoming ∘ slabel <=< get smem) J;
+  do! guard? forallb (set_elem sc) <$>
+               map_options (stag_writers  ∘ slabel <=< get smem) S;
+  Some sc.
+End With_EqType_refined_compartment.
 
-Definition refine_compartment_tag (C   : list (Abs.compartment t))
-                                  (sst : sstate)
-                                  (p   : word) : Prop :=
-  match get (Symbolic.mem sst) p with
+Definition refine_compartment_tag (C : list (Abs.compartment t))
+                                  (M : Sym.memory t)
+                                  (p : word) : Prop :=
+  match get M p with
     | Some (_ @ (Sym.DATA cid I W)) =>
-      (exists c,
-         Abs.in_compartment p C c /\
-         forall p',
-           match get (Symbolic.mem sst) p' with
-             | Some (_ @ (Sym.DATA cid' _ _)) => cid = cid' ->
-                                                 Abs.in_compartment p' C c
-             | Some (_ @ _)                   => False
-             | None                           => True
-           end) /\
-        is_set I /\ is_set W
+      is_set I /\ is_set W /\
+      exists c,
+        C ⊢ p ∈ c /\
+        forall p',
+          match get M p' with
+            | Some (_ @ (Sym.DATA cid' I' W')) =>
+              (cid = cid' <-> C ⊢ p' ∈ c) /\
+              (In cid I'  <-> In p' (Abs.jump_targets  c)) /\
+              (In cid W'  <-> In p' (Abs.shared_memory c))
+            | Some (_ @ _) =>
+              False
+            | None =>
+              True
+          end
     | Some (_ @ _) =>
       False
     | None =>
@@ -110,31 +118,80 @@ Definition refine_compartment_tag (C   : list (Abs.compartment t))
 
 Definition refine_compartments (C : list (Abs.compartment t))
                                (sst : sstate) : Prop :=
-  forallb (refine_compartment_b ^~ (Symbolic.mem sst)) C /\
-  (forall p, refine_compartment_tag C sst p).
+  forallb (is_some ∘ refined_compartment ^~ (Symbolic.mem sst)) C /\
+  forall p, refine_compartment_tag C (Symbolic.mem sst) p.
+
+Definition refine_previous_b (sk : where_from) (prev : Abs.compartment t)
+                             (spc : satom) (SM : Sym.memory t) : bool :=
+  match spc with
+    | _ @ (Sym.PC F cid) => (sk == F) &&
+                            (refined_compartment prev SM == Some cid)
+    | _ @ _ => false
+  end.
 
 Record refine (ast : astate) (sst : sstate) : Prop := RefineState
   { pc_refined           : refine_pc_b         (Abs.pc   ast) (Symbolic.pc   sst)
   ; regs_refined         : refine_registers    (Abs.regs ast) (Symbolic.regs sst)
   ; mems_refined         : refine_memory       (Abs.mem  ast) (Symbolic.mem  sst)
-  ; compartments_refined : refine_compartments (Abs.compartments ast) sst }.
+  ; compartments_refined : refine_compartments (Abs.compartments ast) sst
+  ; previous_refined     : refine_previous_b   (Abs.step_kind ast)
+                                               (Abs.previous  ast)
+                                               (Symbolic.pc   sst)
+                                               (Symbolic.mem  sst) }.
 
 Generalizable All Variables.
+
+Ltac explode_refined_compartment RC A J S :=
+  let sxs      := fresh "sxs"      in
+  let def_sxs  := fresh "def_sxs"  in
+  let sc       := fresh "sc"       in
+  let def_sc   := fresh "def_sc"   in
+  let ALL_J    := fresh "ALL_J"    in
+  let ALL_S    := fresh "ALL_S"    in
+  let mJ       := fresh "mJ"       in
+  let MAP_J    := fresh "MAP_J"    in
+  let mS       := fresh "mS"       in
+  let MAP_S    := fresh "MAP_S"    in
+  let SAME_cid := fresh "SAME_cid" in
+  let TEMP     := fresh "TEMP"     in
+  match type of RC with
+    | refined_compartment ?c _ ?= _ => destruct c as [A J S]
+  end;
+  rewrite /refined_compartment /= in RC;
+     undo1 RC sxs; undo1 RC sc;
+     undo1 RC ALL_J; undo1 RC ALL_S;
+     inversion RC; subst sc; clear RC;
+  let unfmap hyp name eqn :=
+      match type of hyp with
+        | (_ <$> ?opt) = Some _ =>
+          destruct opt as [name|] eqn:eqn;
+            [simpl in hyp | discriminate];
+            let H := fresh hyp in
+            inversion hyp as [H]; clear hyp; rename H into hyp
+      end
+  in unfmap ALL_J mJ MAP_J; unfmap ALL_S mS MAP_S;
+     move/map_options_in in MAP_J; move/map_options_in in MAP_S;
+     rewrite ->forallb_forall in *; simpl in *;
+  move/map_options_in in def_sxs;
+  destruct (map_options _ sxs) as [cids|] eqn:MAP_sxs; simpl in *;
+    [|discriminate];
+  move/map_options_in in MAP_sxs;
+  move: def_sc => /the_spec [NE_cids SAME_cid];
+  unfold SetoidClass.equiv,SetoidDec.eq_setoid in SAME_cid.
 
 Theorem refine_good : forall `(REFINE : refine ast sst),
   Abs.good_state ast ->
   Sym.good_state sst.
 Proof.
   clear S I.
-  intros [Apc AR AM AC Aold]
+  move=> [Apc AR AM AC Ask Aprev]
          [SM SR [Spc Lpc] [Snext]]
-         [RPC RREGS RMEMS RCOMPS]
-         GOOD;
+         [RPC RREGS RMEMS RCOMPS RPREV]
+         /andP [/andP [/andP [ELEM GOODS] SS] SP];
     simpl in *;
     unfold refine_compartments in RCOMPS; simpl in RCOMPS;
     destruct RCOMPS as [RCOMPS RTAGS];
-  unfold Sym.good_state, Abs.good_state in *; simpl in *;
-    move: GOOD => /andP [ICO GOOD].
+  unfold Sym.good_state, Abs.good_state in *; simpl in *.
   repeat split.
   - intros p; unfold Sym.good_memory_tag.
     unfold refine_memory, pointwise in RMEMS; specialize RMEMS with p.
@@ -150,7 +207,22 @@ Proof.
     destruct (get AR r) as [Ax|] eqn:AGET; [|elim RREGS].
     unfold refine_reg_b in RREGS.
     by destruct SL.
-  - by destruct Lpc.
+  - destruct Lpc; try discriminate.
+    move: RPREV => /andP [/eqP? /eqP RPREV]; subst.
+    let S := fresh "S" in explode_refined_compartment RPREV A J S.
+    destruct cids as [|c' cids]; [discriminate | clear NE_cids].
+    specialize (SAME_cid c' (or_introl Logic.eq_refl)); subst.
+    specialize MAP_sxs with c;
+      move: MAP_sxs => [MAP_sxs _];
+      specialize (MAP_sxs (or_introl Logic.eq_refl)).
+    move: MAP_sxs => [[x Lx] [TAG IN]].
+    apply def_sxs in IN.
+    destruct IN as [p [GET IN]].
+    rewrite /refine_memory /pointwise /refine_mem_loc_b in RMEMS.
+    specialize RMEMS with p; rewrite GET in RMEMS.
+    destruct (get AM p); [|done].
+    destruct Lx as [|c' I W|]; try done.
+    simpl in TAG; inversion TAG; subst; clear TAG; eauto.
 Qed.
 
 Ltac unoption :=
@@ -161,23 +233,177 @@ Ltac unoption :=
     | EQ  : None   = None   |- _ => clear EQ
   end.
 
-(* For greppability *)
-Tactic Notation "pni" "admit" :=
-  match goal with
-    | |- Abs.permitted_now_in _ _ _ _ = Some _ => admit
-    | _ => fail 1 "Not a `permitted_now_in' case"
-  end.
+Lemma prove_refined_compartment : forall pc instr cid cid' cid'' I W F
+                                         AR AM AC Ask Aprev c mem,
+  get mem pc ?= instr@(Sym.DATA cid'' I W) ->
+  (do! guard (cid'' == cid') || ((F == JUMPED) && set_elem cid' I);
+   Some cid'') ?= cid ->
+  Abs.good_state (Abs.State pc AR AM AC Ask Aprev) ->
+  forallb (is_some ∘ refined_compartment^~ mem) AC ->
+  (forall p, refine_compartment_tag AC mem p) ->
+  AC ⊢ pc ∈ c ->
+  is_set I ->
+  (forall p' : word,
+     match get mem p' with
+       | Some _@(Sym.PC _ _) => False
+       | Some _@(Sym.DATA cid''' I' W') =>
+         (cid'' = cid''' <-> AC ⊢ p' ∈ c) /\
+         (In cid'' I' <-> In p' (Abs.jump_targets c)) /\
+         (In cid'' W' <-> In p' (Abs.shared_memory c))
+       | Some _@Sym.REG => False
+       | None => True
+     end) ->
+  refined_compartment c mem == Some cid.
+Proof.
+  clear S I; intros until 0;
+    intros PC def_cid AGOOD RCOMPS RCTAGS IN_c SET_I RTAG;
+    rewrite /refine_compartment_tag in RCTAGS; simpl in *;
+    apply/eqP.
+  assert (OK : is_some (refined_compartment c mem)). {
+    move/forallb_forall in RCOMPS. apply RCOMPS.
+    apply Abs.in_compartment_spec in IN_c; tauto.
+  }
+  destruct (refined_compartment c mem) as [cid'''|] eqn:OK';
+    [clear OK; rename OK' into OK; f_equal | discriminate].
+  let S := fresh "S" in explode_refined_compartment OK A J S.
+  undo1 def_cid COND;
+    move: COND => /orP [/eqP? | /andP [/eqP? /set_elem_true IN]];
+                 subst; inversion def_cid; subst; clear def_cid;
+                 [|lapply IN; [clear IN; intros IN | auto]].
+  - move: NE_cids => /nonempty_iff_in [cid' IN_cid].
+    specialize (SAME_cid cid' IN_cid); subst.
+    apply MAP_sxs in IN_cid.
+    move: IN_cid => [[v [F' cid'|cid' I' W'|]] [EQ_cid IN_sxs]];
+                   simpl in *; try discriminate;
+                   inversion EQ_cid; subst; clear EQ_cid;
+                   apply def_sxs in IN_sxs; destruct IN_sxs as [p [GET IN_p]];
+                   [by specialize RTAG with p; rewrite GET in RTAG|].
+    move: (RCTAGS p) => RCTAGS'; rewrite GET in RCTAGS';
+                        move: RCTAGS' => [SET_I' [SET_W' [c [IC_p_c RTAG']]]].
+    assert (IC_p_AJS : AC ⊢ p ∈ <<A,J,S>>) by
+        (apply Abs.in_compartment_spec; apply Abs.in_compartment_spec in IN_c;
+         tauto).
+    assert (c = <<A,J,S>>) by eauto 3; subst.
+    specialize RTAG with p; rewrite GET in RTAG;
+    destruct RTAG as [SAME _].
+    symmetry; apply SAME; assumption.
+  - symmetry; apply SAME_cid.
+    apply MAP_sxs; exists instr@(Sym.DATA cid I W); simpl; split; auto.
+    apply def_sxs.
+    exists pc; split; auto.
+    apply Abs.in_compartment_spec in IN_c; tauto.
+Qed.
+
+Lemma prove_permitted_now_in : forall pc instr cid cid' cid'' I W F
+                                      AR AM AC Ask Aprev
+                                      mem reg int
+                                      c,
+  get mem pc ?= instr@(Sym.DATA cid'' I W) ->
+  (Ask == F) && (refined_compartment Aprev mem == Some cid') ->
+  (do! guard (cid'' == cid') || ((F == JUMPED) && set_elem cid' I);
+   Some cid'') ?= cid ->
+  Abs.good_state (Abs.State pc AR AM AC Ask Aprev) ->
+  Sym.good_state (Symbolic.State (sp := sym_sfi)
+                                 mem reg pc@(Sym.PC F cid') int) ->
+  (forall p, refine_compartment_tag AC mem p) ->
+  AC ⊢ pc ∈ c ->
+  is_set I ->
+  (forall p' : word,
+     match get mem p' with
+      | Some _@(Sym.PC _ _) => False
+      | Some _@(Sym.DATA cid''' I' W') =>
+          (cid'' = cid''' <-> AC ⊢ p' ∈ c) /\
+          (In cid'' I' <-> In p' (Abs.jump_targets c)) /\
+          (In cid'' W' <-> In p' (Abs.shared_memory c))
+      | Some _@Sym.REG => False
+      | None => True
+     end) ->
+  Abs.permitted_now_in AC Ask Aprev pc ?= c.
+Proof.
+  clear S I; intros until 0;
+    intros PC RPREV def_cid AGOOD SGOOD RCTAGS IN_c SET_I RTAG;
+    rewrite /refine_compartment_tag in RCTAGS; simpl in *.
+  eapply Abs.permitted_now_in_spec; eauto 3.
+  split; auto.
+  move: RPREV => /andP [/eqP ? /eqP RPREV]; subst Ask.
+  assert (IN_prev : In Aprev AC). {
+    apply Abs.good_state_decomposed__previous_is_compartment in AGOOD;
+      auto.
+    set (ELT := elem Aprev AC) in *; by destruct ELT.
+  }
+  explode_refined_compartment RPREV Aprev Jprev Sprev.
+  undo1 def_cid COND;
+    move: COND => /orP [/eqP? | /andP [/eqP? /set_elem_true IN]];
+    subst; inversion def_cid; subst; clear def_cid;
+    [ left
+    | right; split; auto; lapply IN; [clear IN; intros IN | auto]].
+  - move: NE_cids => /nonempty_iff_in [cid' IN_cid].
+    specialize (SAME_cid cid' IN_cid); subst.
+    apply MAP_sxs in IN_cid.
+    move: IN_cid => [[v [F' cid'|cid' I' W'|]] [EQ_cid IN_sxs]];
+      simpl in *; try discriminate;
+      inversion EQ_cid; subst; clear EQ_cid;
+      apply def_sxs in IN_sxs; destruct IN_sxs as [p [GET IN_p]];
+      specialize RTAG with p; rewrite GET in RTAG; try done.
+    destruct RTAG as [[SAME _] _].
+    assert (IC_p_c    : AC ⊢ p ∈ c) by auto.
+    assert (IC_p_prev : AC ⊢ p ∈ <<Aprev,Jprev,Sprev>>) by
+      by apply Abs.in_compartment_spec.
+    eauto 3.
+  - rewrite /Sym.good_state /= in SGOOD.
+    move: SGOOD => [[_ [_ [p' [x' [I' [W' GET']]]]]] _].
+    assert (IC'' : AC ⊢ p' ∈ <<Aprev,Jprev,Sprev>>). {
+      move/id in def_sxs; move/id in MAP_sxs;
+        move/id in SAME_cid; move/id in NE_cids.
+      destruct cids as [|cid'' cids];
+        [discriminate | clear NE_cids; simpl in *].
+      move: (SAME_cid cid'' (or_introl Logic.eq_refl)) => ?; subst.
+      move: (MAP_sxs cid') => [MAP_sxs' _];
+        specialize (MAP_sxs' (or_introl Logic.eq_refl)).
+      move: MAP_sxs' => [[v Lv] [TAG IN_sxs]]; simpl in *.
+      apply def_sxs in IN_sxs.
+      destruct IN_sxs as [p [GET_p IN_p]].
+      move: (RCTAGS p) => RTAG'; rewrite GET_p in RTAG'.
+      destruct Lv as [|cid'' I'' W''|]; try done.
+      simpl in TAG; inversion TAG; subst.
+      move: RTAG' => [_ [_ [c'' [IC'' RTAG']]]].
+      specialize RTAG' with p'; rewrite GET' in RTAG';
+        move: RTAG' => [[SAME _] _].
+      specialize (SAME Logic.eq_refl).
+      assert (IC_p_prev : AC ⊢ p ∈ <<Aprev,Jprev,Sprev>>) by
+        by apply Abs.in_compartment_spec.
+      assert (c'' = <<Aprev,Jprev,Sprev>>) by eauto 3; subst.
+      assumption.
+    }
+    move: (RCTAGS p') => RCTAGS'; rewrite GET' in RCTAGS';
+      move: RCTAGS' => [_ [_ [c' [IC' RTAG']]]].
+    specialize RTAG' with pc; rewrite PC in RTAG'.
+    move: RTAG' => [_ [IN_I _]].
+    apply IN_I in IN.
+    by assert (c' = <<Aprev,Jprev,Sprev>>) by eauto 3; subst.
+Qed.
+
+Lemma refined_compartment_preserved : forall mem mem' C,
+  pointwise (fun x x' => slabel x = slabel x') mem mem' ->
+  refined_compartment C mem = refined_compartment C mem'.
+Proof.
+  clear S I; intros mem mem' C SAME.
+  admit.
+Qed.  
 
 (* This *really* needs to be cleaned up! *)
 Theorem backward_simulation : forall ast sst sst',
+  Abs.good_state ast ->
   refine ast sst ->
   sstep sst sst' ->
   exists ast',
     astep ast ast' /\
     refine ast' sst'.
 Proof.
-  clear S I; move=> ast sst sst' REFINE SSTEP.
-  destruct REFINE as [RPC RREGS RMEMS RCOMP], ast as [Apc AR AM AC Aold];
+  clear S I; move=> ast sst sst' AGOOD REFINE SSTEP.
+  assert (SGOOD : Sym.good_state sst) by (eapply refine_good; eassumption).
+  destruct REFINE as [RPC RREGS RMEMS RCOMP RPREV],
+           ast    as [Apc AR    AM    AC    Ask Aprev];
     simpl in *.
   destruct SSTEP; subst; try subst mvec;
     unfold Symbolic.next_state_reg, Symbolic.next_state_pc,
@@ -189,14 +415,14 @@ Proof.
   - (* Nop *)
     undo1 NEXT rvec; undo1 def_rvec cid;
       unfold Sym.can_execute,Sym.sfi_rvec in *; unoption; simpl in *.
-    destruct tpc as [S cid'| |]; try discriminate;
+    destruct tpc as [F cid'| |]; try discriminate;
       destruct ti as [|cid'' I W|]; try discriminate.
     move/eqP in RPC; subst Apc.
     generalize RCOMP;
       rewrite /refine_compartments /refine_compartment_tag /= in RCOMP;
       move: RCOMP => [RCOMPS RCTAGS] RCOMP.
-    specialize RCTAGS with pc; rewrite PC in RCTAGS.
-    destruct RCTAGS as [[c [IN_c IN_SAME]] [SET_I SET_W]].
+    move: (RCTAGS pc) => RCTAGS'; rewrite PC in RCTAGS';
+      destruct RCTAGS' as [SET_I [SET_W [c [IN_c RTAG]]]].
     exists (Abs.State (pc+1)%w AR AM AC INTERNAL c); split.
     + eapply Abs.step_nop; try reflexivity.
       * unfold Abs.decode.
@@ -204,23 +430,24 @@ Proof.
           specialize RMEMS with pc; rewrite PC in RMEMS;
           destruct (get AM pc); [simpl|contradiction].
         move/eqP in RMEMS; subst; assumption.
-      * pni admit.
-    + by constructor; simpl.
+      * eapply prove_permitted_now_in; eassumption.
+    + constructor; simpl;
+        try solve [done | eapply prove_refined_compartment; eassumption].
   - (* Const *)
     undo1 NEXT rvec;
       destruct told as [| |]; try discriminate;
       undo1 def_rvec cid;
       undo1 NEXT regs';
       unfold Sym.can_execute,Sym.sfi_rvec in *; unoption; simpl in *.
-    destruct tpc as [S cid'| |]; try discriminate;
+    destruct tpc as [F cid'| |]; try discriminate;
       destruct ti as [|cid'' I W|]; try discriminate.
     move/eqP in RPC; subst Apc.
     generalize RCOMP;
       rewrite /refine_compartments /refine_compartment_tag /= in RCOMP;
       move: RCOMP => [RCOMPS RCTAGS] RCOMP.
-    specialize RCTAGS with pc; rewrite PC in RCTAGS.
-    destruct RCTAGS as [[c [IN_c IN_SAME]] [SET_I SET_W]].
-    evar (AR' : Abs.registers t);
+    move: (RCTAGS pc) => RCTAGS'; rewrite PC in RCTAGS';
+      destruct RCTAGS' as [SET_I [SET_W [c [IN_c RTAG]]]].
+    evar (AR' : registers t);
       exists (Abs.State (pc+1)%w AR' AM AC INTERNAL c); split;
       subst AR'.
     + eapply Abs.step_const; try reflexivity.
@@ -229,18 +456,18 @@ Proof.
           specialize RMEMS with pc; rewrite PC in RMEMS;
           destruct (get AM pc); [simpl|contradiction].
         move/eqP in RMEMS; subst; eassumption.
-      * pni admit.
+      * eapply prove_permitted_now_in; eassumption.
       * unfold upd; rewrite /refine_registers /pointwise in RREGS;
           specialize RREGS with r.
         destruct (get AR r) eqn:GET;
           [reflexivity | rewrite OLD in RREGS; done].
-    + constructor; simpl; try done.
+    + constructor; simpl;
+        try solve [done | eapply prove_refined_compartment; eassumption].
       rewrite /refine_registers /pointwise in RREGS *; intros r'.
       destruct (r == r') eqn:EQ_r; move/eqP in EQ_r; [subst r'|].
-      * erewrite get_set_eq, get_upd_eq by eauto using reg_map_axioms.
+      * erewrite get_set_eq, get_upd_eq by eauto.
         by unfold refine_reg_b.
-      * erewrite get_set_neq, get_upd_neq with (m' := regs')
-          by eauto using reg_map_axioms.
+      * erewrite get_set_neq, get_upd_neq with (m' := regs') by eauto.
         apply RREGS.
   - (* Mov *)
     undo1 NEXT rvec;
@@ -248,20 +475,20 @@ Proof.
       undo1 def_rvec cid;
       undo1 NEXT regs';
       unfold Sym.can_execute,Sym.sfi_rvec in *; unoption; simpl in *.
-    destruct tpc as [S cid'| |]; try discriminate;
+    destruct tpc as [F cid'| |]; try discriminate;
       destruct ti as [|cid'' I W|]; try discriminate.
     move/eqP in RPC; subst Apc.
     generalize RCOMP;
       rewrite /refine_compartments /refine_compartment_tag /= in RCOMP;
       move: RCOMP => [RCOMPS RCTAGS] RCOMP.
-    specialize RCTAGS with pc; rewrite PC in RCTAGS.
-    destruct RCTAGS as [[c [IN_c IN_SAME]] [SET_I SET_W]].
+    move: (RCTAGS pc) => RCTAGS'; rewrite PC in RCTAGS';
+      destruct RCTAGS' as [SET_I [SET_W [c [IN_c RTAG]]]].
     rewrite /refine_registers /pointwise in RREGS.
     destruct (get AR r1) as [x1|] eqn:GET1;
       [| specialize RREGS with r1; rewrite R1W GET1 in RREGS; done].
     destruct (get AR r2) as [x2|] eqn:GET2;
       [| specialize RREGS with r2; rewrite OLD GET2 in RREGS; done].
-    evar (AR' : Abs.registers t);
+    evar (AR' : registers t);
       exists (Abs.State (pc+1)%w AR' AM AC INTERNAL c); split;
       subst AR'.
     + eapply Abs.step_mov; try reflexivity.
@@ -270,16 +497,16 @@ Proof.
           specialize RMEMS with pc; rewrite PC in RMEMS;
           destruct (get AM pc); [simpl|contradiction].
         move/eqP in RMEMS; subst; eassumption.
-      * pni admit.
+      * eapply prove_permitted_now_in; eassumption.
       * eassumption.
       * unfold upd; rewrite GET2; reflexivity.
-    + constructor; simpl; try done.
+    + constructor; simpl;
+        try solve [done | eapply prove_refined_compartment; eassumption].
       rewrite /refine_registers /pointwise in RREGS *; intros r2'.
       destruct (r2 == r2') eqn:EQ_r2; move/eqP in EQ_r2; [subst r2'|].
-      * erewrite get_set_eq, get_upd_eq by eauto using reg_map_axioms.
+      * erewrite get_set_eq, get_upd_eq by eauto.
         by specialize RREGS with r1; rewrite GET1 R1W /refine_reg_b in RREGS *.
-      * erewrite get_set_neq, get_upd_neq with (m' := regs')
-          by eauto using reg_map_axioms.
+      * erewrite get_set_neq, get_upd_neq with (m' := regs') by eauto.
         apply RREGS.
   - (* Binop *)
     undo1 NEXT rvec;
@@ -287,14 +514,14 @@ Proof.
       undo1 def_rvec cid;
       undo1 NEXT regs';
       unfold Sym.can_execute,Sym.sfi_rvec in *; unoption; simpl in *.
-    destruct tpc as [S cid'| |]; try discriminate;
+    destruct tpc as [F cid'| |]; try discriminate;
       destruct ti as [|cid'' I W|]; try discriminate.
     move/eqP in RPC; subst Apc.
     generalize RCOMP;
       rewrite /refine_compartments /refine_compartment_tag /= in RCOMP;
       move: RCOMP => [RCOMPS RCTAGS] RCOMP.
-    specialize RCTAGS with pc; rewrite PC in RCTAGS.
-    destruct RCTAGS as [[c [IN_c IN_SAME]] [SET_I SET_W]].
+    move: (RCTAGS pc) => RCTAGS'; rewrite PC in RCTAGS';
+      destruct RCTAGS' as [SET_I [SET_W [c [IN_c RTAG]]]].
     rewrite /refine_registers /pointwise in RREGS.
     destruct (get AR r1) as [x1|] eqn:GET1;
       [| specialize RREGS with r1; rewrite R1W GET1 in RREGS; done].
@@ -302,7 +529,7 @@ Proof.
       [| specialize RREGS with r2; rewrite R2W GET2 in RREGS; done].
     destruct (get AR r3) as [x3|] eqn:GET3;
       [| specialize RREGS with r3; rewrite OLD GET3 in RREGS; done].
-    evar (AR' : Abs.registers t);
+    evar (AR' : registers t);
       exists (Abs.State (pc+1)%w AR' AM AC INTERNAL c); split;
       subst AR'.
     + eapply Abs.step_binop; try reflexivity.
@@ -311,21 +538,21 @@ Proof.
           specialize RMEMS with pc; rewrite PC in RMEMS;
           destruct (get AM pc); [simpl|contradiction].
         move/eqP in RMEMS; subst; eassumption.
-      * pni admit.
+      * eapply prove_permitted_now_in; eassumption.
       * eassumption.
       * eassumption.
       * unfold upd; rewrite GET3; reflexivity.
-    + constructor; simpl; try done.
+    + constructor; simpl;
+        try solve [done | eapply prove_refined_compartment; eassumption].
       unfold upd; rewrite /refine_registers /pointwise in RREGS *; intros r3'.
       destruct (r3 == r3') eqn:EQ_r3; move/eqP in EQ_r3; [subst r3'|].
-      * erewrite get_set_eq, get_upd_eq by eauto using reg_map_axioms.
+      * erewrite get_set_eq, get_upd_eq by eauto.
         { unfold refine_reg_b. apply/eqP; f_equal.
           - by specialize RREGS with r1;
                rewrite GET1 R1W /refine_reg_b in RREGS *; apply/eqP.
           - by specialize RREGS with r2;
                rewrite GET2 R2W /refine_reg_b in RREGS *; apply/eqP. }
-      * erewrite get_set_neq, get_upd_neq with (m' := regs')
-          by eauto using reg_map_axioms.
+      * erewrite get_set_neq, get_upd_neq with (m' := regs') by eauto.
         apply RREGS.
   - (* Load *)
     undo1 NEXT rvec;
@@ -333,14 +560,14 @@ Proof.
       undo1 def_rvec cid;
       undo1 NEXT regs';
       unfold Sym.can_execute,Sym.sfi_rvec in *; unoption; simpl in *.
-    destruct tpc as [S cid'| |]; try discriminate;
+    destruct tpc as [F cid'| |]; try discriminate;
       destruct ti as [|cid'' I'' W''|]; try discriminate.
     move/eqP in RPC; subst Apc.
     generalize RCOMP;
       rewrite /refine_compartments /refine_compartment_tag /= in RCOMP;
       move: RCOMP => [RCOMPS RCTAGS] RCOMP.
-    specialize RCTAGS with pc; rewrite PC in RCTAGS.
-    destruct RCTAGS as [[ac [IN_ac IN_SAME]] [SET_I SET_W]].
+    move: (RCTAGS pc) => RCTAGS'; rewrite PC in RCTAGS';
+      destruct RCTAGS' as [SET_I [SET_W [ac [IN_ac RTAG]]]].
     rewrite /refine_registers /refine_memory /pointwise  in RREGS RMEMS.
     destruct (get AR r1) as [x1|] eqn:GET1;
       [| specialize RREGS with r1; rewrite R1W GET1 in RREGS; done].
@@ -352,7 +579,7 @@ Proof.
       subst x1.
     destruct (get AM w1) as [x2|] eqn:GETM1;
       [|specialize RMEMS with w1; rewrite MEM1 GETM1 in RMEMS; done].
-    evar (AR' : Abs.registers t);
+    evar (AR' : registers t);
       exists (Abs.State (pc+1)%w AR' AM AC INTERNAL ac); split;
       subst AR'.
     + eapply Abs.step_load; try reflexivity.
@@ -361,36 +588,139 @@ Proof.
           specialize RMEMS with pc; rewrite PC in RMEMS;
           destruct (get AM pc); [simpl|contradiction].
         move/eqP in RMEMS; subst; eassumption.
-      * pni admit.
+      * eapply prove_permitted_now_in; eassumption.
       * eassumption.
       * eassumption.
       * unfold upd; rewrite GET2; reflexivity.
-    + constructor; simpl; try done.
+    + constructor; simpl;
+        try solve [ done
+                  | eapply prove_refined_compartment;
+                    (* eassumption picked the wrong thing first *)
+                    try apply def_cid; eassumption].
       unfold upd; rewrite /refine_registers /pointwise in RREGS *; intros r2'.
       destruct (r2 == r2') eqn:EQ_r2; move/eqP in EQ_r2; [subst r2'|].
-      * erewrite get_set_eq, get_upd_eq by eauto using reg_map_axioms.
+      * erewrite get_set_eq, get_upd_eq by eauto.
         by specialize RMEMS with w1;
            rewrite GETM1 MEM1 /refine_mem_loc_b /refine_reg_b in RMEMS *.
-      * erewrite get_set_neq, get_upd_neq with (m' := regs')
-          by eauto using reg_map_axioms.
+      * erewrite get_set_neq, get_upd_neq with (m' := regs') by eauto.
         apply RREGS.
   - (* Store *)
-    admit.
+    undo1 NEXT rvec;
+      destruct t1,t2,told; try discriminate;
+      undo1 def_rvec cid;
+      undo1 def_rvec WRITE_OK;
+      undo1 NEXT mem';
+      unfold Sym.can_execute,Sym.sfi_rvec in *; unoption; simpl in *.
+    destruct tpc as [F cid'| |]; try discriminate;
+      destruct ti as [|cid'' I'' W''|]; try discriminate.
+    move/eqP in RPC; subst Apc.
+    generalize RCOMP;
+      rewrite /refine_compartments /refine_compartment_tag /= in RCOMP;
+      move: RCOMP => [RCOMPS RCTAGS] RCOMP.
+    move: (RCTAGS pc) => RCTAGS'; rewrite PC in RCTAGS';
+      destruct RCTAGS' as [SET_I'' [SET_W'' [ac [IN_ac RTAG]]]].
+    rewrite /refine_registers /refine_memory /pointwise  in RREGS RMEMS.
+    destruct (get AR r1) as [x1|] eqn:GET1;
+      [| specialize RREGS with r1; rewrite R1W GET1 in RREGS; done].
+    destruct (get AR r2) as [x2|] eqn:GET2;
+      [| specialize RREGS with r2; rewrite R2W GET2 in RREGS; done].
+    assert (EQ1 : x1 = w1) by
+      (by specialize RREGS with r1;
+          rewrite R1W GET1 /refine_reg_b in RREGS; move/eqP in RREGS);
+      subst x1.
+    assert (EQ1 : x2 = w2) by
+      (by specialize RREGS with r2;
+          rewrite R2W GET2 /refine_reg_b in RREGS; move/eqP in RREGS);
+      subst x2.
+    destruct (get AM w1) as [xold|] eqn:GETM1;
+      [|specialize RMEMS with w1; rewrite OLD GETM1 in RMEMS; done].
+    evar (AM' : memory t);
+      exists (Abs.State (pc+1)%w AR AM' AC INTERNAL ac); split;
+      subst AM'.
+    + eapply Abs.step_store; try reflexivity.
+      * unfold Abs.decode.
+        unfold refine_memory,pointwise,refine_mem_loc_b in RMEMS;
+          specialize RMEMS with pc; rewrite PC in RMEMS;
+          destruct (get AM pc); [simpl|contradiction].
+        move/eqP in RMEMS; subst; eassumption.
+      * eapply prove_permitted_now_in; eassumption.
+      * eassumption.
+      * eassumption.
+      * { undo1 def_cid COND; unoption.
+          specialize RTAG with w1; rewrite OLD in RTAG.
+          move: RTAG => [[SAME _] [_ [IN_W _]]].
+          apply in_app_iff; move: WRITE_OK => /orP [/eqP? | ELEM];
+            subst; [left | right].
+        - specialize (SAME Logic.eq_refl);
+           apply Abs.in_compartment_spec in SAME;
+           tauto.
+        - apply set_elem_true in ELEM; auto.
+          move: SGOOD => [[SMEM _] _].
+          specialize SMEM with w1; rewrite /Sym.good_memory_tag OLD in SMEM.
+          by move: SMEM => /andP []. }
+      * unfold upd; rewrite GETM1; reflexivity.
+    + assert (SAME : pointwise (fun x x' => slabel x = slabel x') mem mem'). {
+        rewrite /pointwise; intros p.
+        destruct (p == w1) eqn:EQ_w1; move/eqP in EQ_w1; [subst p|].
+        - apply get_upd_eq in def_mem'; auto.
+          by rewrite OLD def_mem'.
+        - apply get_upd_neq with (key' := p) in def_mem'; auto.
+          by rewrite def_mem'; destruct (get mem p).
+      }
+      constructor; simpl; try done.
+      * { unfold upd;
+            rewrite /refine_memory /refine_mem_loc_b /pointwise in RMEMS *;
+            intros p.
+        destruct (p == w1) eqn:EQ_w1; move/eqP in EQ_w1; [subst p|].
+        - erewrite get_set_eq, get_upd_eq by eauto using word_map_axioms.
+          by specialize RMEMS with w1; rewrite GETM1 in RMEMS *.
+        - erewrite get_set_neq, get_upd_neq with (m' := mem')
+            by eauto using word_map_axioms.
+          apply RMEMS. }
+      * { unfold refine_compartments; simpl; split.
+        - apply forallb_forall; intros ac' IN.
+          erewrite <-refined_compartment_preserved; [|eassumption].
+          move/forallb_forall in RCOMPS; auto.
+        - intros p; unfold refine_compartment_tag.
+          generalize def_mem' => def_mem''.
+          destruct (p == w1) eqn:EQ_w1; move/eqP in EQ_w1; [subst p|].
+          + apply get_upd_eq in def_mem'; auto.
+            specialize RCTAGS with w1; rewrite OLD in RCTAGS.
+            move: RCTAGS => [SET_I [SET_W [ac' [IC' RTAG']]]].
+            rewrite def_mem'; repeat split; auto.
+            exists ac'; split; auto.
+            intros p'; specialize RTAG' with p'.
+            destruct (p' == w1) eqn:EQ_w1'; move/eqP in EQ_w1'; [subst p'|].
+            * rewrite OLD in RTAG'; rewrite def_mem'; assumption.
+            * apply get_upd_neq with (key' := p') in def_mem''; auto.
+              rewrite def_mem''; assumption.
+          + apply get_upd_neq with (key' := p) in def_mem'; auto.
+            specialize RCTAGS with p; rewrite def_mem'.
+            destruct (get mem p) as [[? []]|]; auto.
+            move: RCTAGS => [SET_I [SET_W [ac' [IC' RTAG']]]].
+            repeat split; auto.
+            exists ac'; split; auto.
+            intros p'; specialize RTAG' with p'.
+            destruct (p' == w1) eqn:EQ_w1'; move/eqP in EQ_w1'; [subst p'|].
+            * apply get_upd_eq in def_mem''; auto.
+              rewrite OLD in RTAG'; rewrite def_mem''; assumption.
+            * apply get_upd_neq with (key' := p') in def_mem''; auto.
+              rewrite def_mem''; assumption. }
+      * erewrite <-refined_compartment_preserved; [|eassumption].
+        eapply prove_refined_compartment; try apply def_cid; eassumption.
   - (* Jump *)
-    admit.
-  - (* Bnz *)
     undo1 NEXT rvec;
       destruct t1; try discriminate;
       undo1 def_rvec cid;
       unfold Sym.can_execute,Sym.sfi_rvec in *; unoption; simpl in *.
-    destruct tpc as [S cid'| |]; try discriminate;
+    destruct tpc as [F cid'| |]; try discriminate;
       destruct ti as [|cid'' I W|]; try discriminate.
     move/eqP in RPC; subst Apc.
     generalize RCOMP;
       rewrite /refine_compartments /refine_compartment_tag /= in RCOMP;
       move: RCOMP => [RCOMPS RCTAGS] RCOMP.
-    specialize RCTAGS with pc; rewrite PC in RCTAGS.
-    destruct RCTAGS as [[c [IN_c IN_SAME]] [SET_I SET_W]].
+    move: (RCTAGS pc) => RCTAGS'; rewrite PC in RCTAGS';
+      destruct RCTAGS' as [SET_I [SET_W [c [IN_c RTAG]]]].
     rewrite /refine_registers /pointwise in RREGS.
     destruct (get AR r) as [x|] eqn:GET;
       [| specialize RREGS with r; rewrite RW GET in RREGS; done].
@@ -398,7 +728,40 @@ Proof.
       (by specialize RREGS with r;
           rewrite RW GET /refine_reg_b in RREGS; move/eqP in RREGS);
       subst x.
-    evar (AR' : Abs.registers t);
+    evar (AR' : registers t);
+      exists (Abs.State w AR' AM AC JUMPED c); split;
+      subst AR'.
+    + eapply Abs.step_jump; try reflexivity.
+      * unfold Abs.decode.
+        unfold refine_memory,pointwise,refine_mem_loc_b in RMEMS;
+          specialize RMEMS with pc; rewrite PC in RMEMS;
+          destruct (get AM pc); [simpl|contradiction].
+        move/eqP in RMEMS; subst; eassumption.
+      * eapply prove_permitted_now_in; eassumption.
+      * assumption.
+    + constructor; simpl;
+        try solve [done | eapply prove_refined_compartment; eassumption].
+  - (* Bnz *)
+    undo1 NEXT rvec;
+      destruct t1; try discriminate;
+      undo1 def_rvec cid;
+      unfold Sym.can_execute,Sym.sfi_rvec in *; unoption; simpl in *.
+    destruct tpc as [F cid'| |]; try discriminate;
+      destruct ti as [|cid'' I W|]; try discriminate.
+    move/eqP in RPC; subst Apc.
+    generalize RCOMP;
+      rewrite /refine_compartments /refine_compartment_tag /= in RCOMP;
+      move: RCOMP => [RCOMPS RCTAGS] RCOMP.
+    move: (RCTAGS pc) => RCTAGS'; rewrite PC in RCTAGS';
+      destruct RCTAGS' as [SET_I [SET_W [c [IN_c RTAG]]]].
+    rewrite /refine_registers /pointwise in RREGS.
+    destruct (get AR r) as [x|] eqn:GET;
+      [| specialize RREGS with r; rewrite RW GET in RREGS; done].
+    assert (EQ : x = w) by
+      (by specialize RREGS with r;
+          rewrite RW GET /refine_reg_b in RREGS; move/eqP in RREGS);
+      subst x.
+    evar (AR' : registers t);
       exists (Abs.State (pc + (if w == 0 then 1 else imm_to_word n))%w
                         AR' AM AC INTERNAL c); split;
       subst AR'.
@@ -409,10 +772,57 @@ Proof.
           destruct (get AM pc); [simpl|contradiction].
         move/eqP in RMEMS; subst; eassumption.
       * eassumption.
-      * pni admit.
-    + by constructor; simpl.
+      * eapply prove_permitted_now_in; eassumption.
+    + constructor; simpl;
+        try solve [done | eapply prove_refined_compartment; eassumption].
   - (* Jal *)
-    admit.
+    undo1 NEXT rvec;
+      destruct t1; try discriminate;
+      destruct told; try discriminate;
+      undo1 def_rvec cid;
+      undo1 NEXT regs';
+      unfold Sym.can_execute,Sym.sfi_rvec in *; unoption; simpl in *.
+    destruct tpc as [F cid'| |]; try discriminate;
+      destruct ti as [|cid'' I W|]; try discriminate.
+    move/eqP in RPC; subst Apc.
+    generalize RCOMP;
+      rewrite /refine_compartments /refine_compartment_tag /= in RCOMP;
+      move: RCOMP => [RCOMPS RCTAGS] RCOMP.
+    move: (RCTAGS pc) => RCTAGS'; rewrite PC in RCTAGS';
+      destruct RCTAGS' as [SET_I [SET_W [c [IN_c RTAG]]]].
+    rewrite /refine_registers /pointwise in RREGS.
+    destruct (get AR r) as [x|] eqn:GET;
+      [| specialize RREGS with r; rewrite RW GET in RREGS; done].
+    assert (EQ : x = w) by
+      (by specialize RREGS with r;
+          rewrite RW GET /refine_reg_b in RREGS; move/eqP in RREGS);
+      subst x.
+    evar (AR' : registers t);
+      exists (Abs.State w AR' AM AC JUMPED c); split;
+      subst AR'.
+    + eapply Abs.step_jal; try reflexivity.
+      * unfold Abs.decode.
+        unfold refine_memory,pointwise,refine_mem_loc_b in RMEMS;
+          specialize RMEMS with pc; rewrite PC in RMEMS;
+          destruct (get AM pc); [simpl|contradiction].
+        move/eqP in RMEMS; subst; eassumption.
+      * eapply prove_permitted_now_in; eassumption.
+      * assumption.
+      * unfold upd; rewrite /refine_registers /pointwise in RREGS.
+        match goal with |- context[get AR ?ra] =>
+          (* This finds the type class instances *)
+          specialize RREGS with ra;
+          destruct (get AR ra) eqn:GET';
+            [reflexivity | rewrite OLD in RREGS; done]
+        end.
+    + constructor; simpl;
+        try solve [done | eapply prove_refined_compartment; eassumption].
+      rewrite /refine_registers /pointwise in RREGS *; intros r'.
+      destruct (ra == r') eqn:EQ_r'; move/eqP in EQ_r'; [subst r'|].
+      * erewrite get_set_eq, get_upd_eq by eauto.
+        by simpl.
+      * erewrite get_set_neq, get_upd_neq with (m' := regs') by eauto.
+        apply RREGS.
   - (* Syscall *)
     admit.
 Qed.
