sfi/common.v
@@ -27,3 +27,5 @@ Proof. by move=> [|] [|] /=; apply: (iffP idP). Qed.
 
 Definition where_from_eqMixin := EqMixin where_from_eqP.
 Canonical where_from_eqType := Eval hnf in EqType where_from where_from_eqMixin.
+
+Notation "x ?= y" := (x = Some y) (at level 70, no associativity).
